ported the new stacking proof with the new cc_stacking definition

backend/Stackingproof.v
@@ -21,6 +21,7 @@ Require Import LTL Op Locations Linear Mach.
 Require Import Bounds Conventions Stacklayout Lineartyping.
 Require Import Stacking.
 Require Import LanguageInterface Invariant cklr.Inject cklr.InjectFootprint.
+Require CallConv.
 
 Local Open Scope sep_scope.
 Local Opaque Z.add Z.mul Z.divide.
@@ -349,38 +350,41 @@ Qed.
   up to the memory injection [j].  The memory layout of the registers in [rl]
   is the same as that implemented by [save_callee_save_rec]. *)
 
-Fixpoint contains_callee_saves (j: meminj) (sp: block) (pos: Z) (rl: list mreg) (ls: locset) : massert :=
+
+Fixpoint contains_callee_saves (j: meminj) (sp: block) (pos: Z) (rl: list mreg) (ls: locset) (rs: regset) : massert :=
   match rl with
   | nil => pure True
   | r :: rl =>
       let ty := mreg_type r in
       let sz := AST.typesize ty in
       let pos1 := align pos sz in
-      contains (chunk_of_type ty) sp pos1 (fun v => Val.inject j (ls (R r)) v)
-      ** contains_callee_saves j sp (pos1 + sz) rl ls
+      contains (chunk_of_type ty) sp pos1 (fun v => Val.inject j (ls (R r)) v /\ rs r = v)
+      ** contains_callee_saves j sp (pos1 + sz) rl ls rs
   end.
 
 Lemma contains_callee_saves_incr:
-  forall j j' sp ls,
+  forall j j' sp ls rs,
   inject_incr j j' ->
   forall rl pos,
-  massert_imp (contains_callee_saves j sp pos rl ls)
-              (contains_callee_saves j' sp pos rl ls).
+  massert_imp (contains_callee_saves j sp pos rl ls rs)
+              (contains_callee_saves j' sp pos rl ls rs).
 Proof.
   induction rl as [ | r1 rl]; simpl; intros.
 - reflexivity.
-- apply sepconj_morph_1; auto. apply contains_imp. eauto.
+- apply sepconj_morph_1; auto. apply contains_imp.
+  intros v [A B]. split; eauto.
 Qed.
 
 Lemma contains_callee_saves_exten:
-  forall j sp ls ls' rl pos,
-  (forall r, In r rl -> ls' (R r) = ls (R r)) ->
-  massert_eqv (contains_callee_saves j sp pos rl ls)
-              (contains_callee_saves j sp pos rl ls').
+  forall j sp ls ls' rl pos rs rs',
+    (forall r, In r rl -> ls' (R r) = ls (R r)) ->
+    (forall r, In r rl -> rs' r = rs r) ->
+  massert_eqv (contains_callee_saves j sp pos rl ls rs)
+              (contains_callee_saves j sp pos rl ls' rs').
 Proof.
   induction rl as [ | r1 rl]; simpl; intros.
 - reflexivity.
-- apply sepconj_morph_2; auto. rewrite H by auto. reflexivity.
+- apply sepconj_morph_2; auto. rewrite H by auto. rewrite H0 by auto. reflexivity.
 Qed.
 
 (** Separation logic assertions describing the stack frame at [sp].
@@ -396,23 +400,24 @@ In addition, we use a nonseparating conjunction to record the fact that
 we have full access rights on the stack frame, except the part that
 represents the Linear stack data. *)
 
-Definition frame_contents_1 (j: meminj) (sp: block) (ls ls0: locset) (parent retaddr: val) :=
+Definition frame_contents_1 (j: meminj) (sp: block) (ls ls0: locset) (rs0: regset) (parent retaddr: val) :=
     contains_locations j sp fe.(fe_ofs_local) b.(bound_local) Local ls
  ** contains_locations j sp fe_ofs_arg b.(bound_outgoing) Outgoing ls
  ** hasvalue Mptr sp fe.(fe_ofs_link) parent
  ** hasvalue Mptr sp fe.(fe_ofs_retaddr) retaddr
- ** contains_callee_saves j sp fe.(fe_ofs_callee_save) b.(used_callee_save) ls0.
+ ** contains_callee_saves j sp fe.(fe_ofs_callee_save) b.(used_callee_save) ls0 rs0.
 
-Definition frame_contents (j: meminj) (sp: block) (ls ls0: locset) (parent retaddr: val) :=
-  mconj (frame_contents_1 j sp ls ls0 parent retaddr)
+Definition frame_contents (j: meminj) (sp: block) (ls ls0: locset) (rs0 : regset) (parent retaddr: val) :=
+  mconj (frame_contents_1 j sp ls ls0 rs0 parent retaddr)
         (range sp 0 fe.(fe_stack_data) **
          range sp (fe.(fe_stack_data) + b.(bound_stack_data)) fe.(fe_size)).
 
 (** Accessing components of the frame. *)
 
+
 Lemma frame_get_local:
-  forall ofs ty j sp ls ls0 parent retaddr m P,
-  m |= frame_contents j sp ls ls0 parent retaddr ** P ->
+  forall ofs ty j sp ls ls0 rs0 parent retaddr m P,
+  m |= frame_contents j sp ls ls0 rs0 parent retaddr ** P ->
   slot_within_bounds b Local ofs ty -> slot_valid f Local ofs ty = true ->
   exists v,
      load_stack m (Vptr sp Ptrofs.zero) ty (Ptrofs.repr (offset_local fe ofs)) = Some v
@@ -424,8 +429,8 @@ Proof.
 Qed.
 
 Lemma frame_get_outgoing:
-  forall ofs ty j sp ls ls0 parent retaddr m P,
-  m |= frame_contents j sp ls ls0 parent retaddr ** P ->
+  forall ofs ty j sp ls ls0 rs0 parent retaddr m P,
+  m |= frame_contents j sp ls ls0 rs0 parent retaddr ** P ->
   slot_within_bounds b Outgoing ofs ty -> slot_valid f Outgoing ofs ty = true ->
   exists v,
      load_stack m (Vptr sp Ptrofs.zero) ty (Ptrofs.repr (offset_arg ofs)) = Some v
@@ -437,8 +442,8 @@ Proof.
 Qed.
 
 Lemma frame_get_parent:
-  forall j sp ls ls0 parent retaddr m P,
-  m |= frame_contents j sp ls ls0 parent retaddr ** P ->
+  forall j sp ls ls0 rs0 parent retaddr m P,
+  m |= frame_contents j sp ls ls0 rs0 parent retaddr ** P ->
   load_stack m (Vptr sp Ptrofs.zero) Tptr (Ptrofs.repr fe.(fe_ofs_link)) = Some parent.
 Proof.
   unfold frame_contents, frame_contents_1; intros.
@@ -447,8 +452,8 @@ Proof.
 Qed.
 
 Lemma frame_get_retaddr:
-  forall j sp ls ls0 parent retaddr m P,
-  m |= frame_contents j sp ls ls0 parent retaddr ** P ->
+  forall j sp ls ls0 rs0 parent retaddr m P,
+  m |= frame_contents j sp ls ls0 rs0 parent retaddr ** P ->
   load_stack m (Vptr sp Ptrofs.zero) Tptr (Ptrofs.repr fe.(fe_ofs_retaddr)) = Some retaddr.
 Proof.
   unfold frame_contents, frame_contents_1; intros.
@@ -458,14 +463,15 @@ Qed.
 
 (** Assigning a [Local] or [Outgoing] stack slot. *)
 
+
 Lemma frame_set_local:
-  forall ofs ty v v' j sp ls ls0 parent retaddr m P,
-  m |= frame_contents j sp ls ls0 parent retaddr ** P ->
+  forall ofs ty v v' j sp ls ls0 rs0 parent retaddr m P,
+  m |= frame_contents j sp ls ls0 rs0 parent retaddr ** P ->
   slot_within_bounds b Local ofs ty -> slot_valid f Local ofs ty = true ->
   Val.inject j v v' ->
   exists m',
      store_stack m (Vptr sp Ptrofs.zero) ty (Ptrofs.repr (offset_local fe ofs)) v' = Some m'
-  /\ m' |= frame_contents j sp (Locmap.set (S Local ofs ty) v ls) ls0 parent retaddr ** P.
+  /\ m' |= frame_contents j sp (Locmap.set (S Local ofs ty) v ls) ls0 rs0 parent retaddr ** P.
 Proof.
   intros. unfold frame_contents in H.
   exploit mconj_proj1; eauto. unfold frame_contents_1.
@@ -484,13 +490,13 @@ Proof.
 Qed.
 
 Lemma frame_set_outgoing:
-  forall ofs ty v v' j sp ls ls0 parent retaddr m P,
-  m |= frame_contents j sp ls ls0 parent retaddr ** P ->
+  forall ofs ty v v' j sp ls ls0 rs0 parent retaddr m P,
+  m |= frame_contents j sp ls ls0 rs0 parent retaddr ** P ->
   slot_within_bounds b Outgoing ofs ty -> slot_valid f Outgoing ofs ty = true ->
   Val.inject j v v' ->
   exists m',
      store_stack m (Vptr sp Ptrofs.zero) ty (Ptrofs.repr (offset_arg ofs)) v' = Some m'
-  /\ m' |= frame_contents j sp (Locmap.set (S Outgoing ofs ty) v ls) ls0 parent retaddr ** P.
+  /\ m' |= frame_contents j sp (Locmap.set (S Outgoing ofs ty) v ls) ls0 rs0 parent retaddr ** P.
 Proof.
   intros. unfold frame_contents in H.
   exploit mconj_proj1; eauto. unfold frame_contents_1.
@@ -511,12 +517,13 @@ Qed.
 (** Invariance by change of location maps. *)
 
 Lemma frame_contents_exten:
-  forall ls ls0 ls' ls0' j sp parent retaddr P m,
+  forall ls ls0 ls' ls0' rs0 rs0' j sp parent retaddr P m,
   (forall ofs ty, Val.lessdef (ls' (S Local ofs ty)) (ls (S Local ofs ty))) ->
   (forall ofs ty, Val.lessdef (ls' (S Outgoing ofs ty)) (ls (S Outgoing ofs ty))) ->
   (forall r, In r b.(used_callee_save) -> ls0' (R r) = ls0 (R r)) ->
-  m |= frame_contents j sp ls ls0 parent retaddr ** P ->
-  m |= frame_contents j sp ls' ls0' parent retaddr ** P.
+  (forall r, In r b.(used_callee_save) -> rs0' r = rs0 r) ->
+  m |= frame_contents j sp ls ls0 rs0 parent retaddr ** P ->
+  m |= frame_contents j sp ls' ls0' rs0' parent retaddr ** P.
 Proof.
   unfold frame_contents, frame_contents_1; intros.
   rewrite <- ! (contains_locations_exten ls ls') by auto.
@@ -526,18 +533,19 @@ Qed.
 
 (** Invariance by assignment to registers. *)
 
+
 Corollary frame_set_reg:
-  forall r v j sp ls ls0 parent retaddr m P,
-  m |= frame_contents j sp ls ls0 parent retaddr ** P ->
-  m |= frame_contents j sp (Locmap.set (R r) v ls) ls0 parent retaddr ** P.
+  forall r v j sp ls ls0 rs0 parent retaddr m P,
+  m |= frame_contents j sp ls ls0 rs0 parent retaddr ** P ->
+  m |= frame_contents j sp (Locmap.set (R r) v ls) ls0 rs0 parent retaddr ** P.
 Proof.
-  intros. apply frame_contents_exten with ls ls0; auto.
+  intros. eapply frame_contents_exten; eauto.
 Qed.
 
 Corollary frame_undef_regs:
-  forall j sp ls ls0 parent retaddr m P rl,
-  m |= frame_contents j sp ls ls0 parent retaddr ** P ->
-  m |= frame_contents j sp (LTL.undef_regs rl ls) ls0 parent retaddr ** P.
+  forall j sp ls ls0 rs0 parent retaddr m P rl,
+  m |= frame_contents j sp ls ls0 rs0 parent retaddr ** P ->
+  m |= frame_contents j sp (LTL.undef_regs rl ls) ls0 rs0 parent retaddr ** P.
 Proof.
 Local Opaque sepconj.
   induction rl; simpl; intros.
@@ -545,10 +553,21 @@ Local Opaque sepconj.
 - apply frame_set_reg; auto.
 Qed.
 
+Corollary frame_callee_save_eq:
+  forall j sp ls ls0 rs0 rs0' parent retaddr m P,
+    m |= frame_contents j sp ls ls0 rs0 parent retaddr ** P ->
+    (forall r, is_callee_save r = true -> rs0 r = rs0' r) ->
+    m |= frame_contents j sp ls ls0 rs0' parent retaddr ** P.
+Proof.
+  intros. eapply frame_contents_exten. eauto. eauto. 3: eauto.
+  eauto. intros. rewrite <- H0; eauto.
+  eapply used_callee_save_prop; eauto.
+Qed.
+
 Corollary frame_set_regpair:
-  forall j sp ls0 parent retaddr m P p v ls,
-  m |= frame_contents j sp ls ls0 parent retaddr ** P ->
-  m |= frame_contents j sp (Locmap.setpair p v ls) ls0 parent retaddr ** P.
+  forall j sp ls0 rs0 parent retaddr m P p v ls,
+  m |= frame_contents j sp ls ls0 rs0 parent retaddr ** P ->
+  m |= frame_contents j sp (Locmap.setpair p v ls) ls0 rs0 parent retaddr ** P.
 Proof.
   intros. destruct p; simpl.
   apply frame_set_reg; auto.
@@ -556,9 +575,9 @@ Proof.
 Qed.
 
 Corollary frame_set_res:
-  forall j sp ls0 parent retaddr m P res v ls,
-  m |= frame_contents j sp ls ls0 parent retaddr ** P ->
-  m |= frame_contents j sp (Locmap.setres res v ls) ls0 parent retaddr ** P.
+  forall j sp ls0 rs0 parent retaddr m P res v ls,
+  m |= frame_contents j sp ls ls0 rs0 parent retaddr ** P ->
+  m |= frame_contents j sp (Locmap.setres res v ls) ls0 rs0 parent retaddr ** P.
 Proof.
   induction res; simpl; intros.
 - apply frame_set_reg; auto.
@@ -569,10 +588,10 @@ Qed.
 (** Invariance by change of memory injection. *)
 
 Lemma frame_contents_incr:
-  forall j sp ls ls0 parent retaddr m P j',
-  m |= frame_contents j sp ls ls0 parent retaddr ** P ->
+  forall j sp ls ls0 rs0 parent retaddr m P j',
+  m |= frame_contents j sp ls ls0 rs0 parent retaddr ** P ->
   inject_incr j j' ->
-  m |= frame_contents j' sp ls ls0 parent retaddr ** P.
+  m |= frame_contents j' sp ls ls0 rs0 parent retaddr ** P.
 Proof.
   unfold frame_contents, frame_contents_1; intros.
   rewrite <- (contains_locations_incr j j') by auto.
@@ -580,6 +599,7 @@ Proof.
   erewrite  <- contains_callee_saves_incr by eauto.
   assumption.
 Qed.
+
 
 (** * Agreement between location sets and Mach states *)
 
@@ -749,6 +769,14 @@ Proof.
   intros; red; intros. congruence.
 Qed.
 
+Lemma reg_within_bounds_caller_save:
+  forall r,
+  ~ mreg_within_bounds b r -> is_callee_save r = true.
+Proof.
+  intros. destruct (is_callee_save r) eqn:?; eauto.
+  elim H. red. intros. congruence.
+Qed.
+
 Lemma agree_locs_set_pair:
   forall ls0 p v ls,
   agree_locs ls ls0 ->
@@ -833,6 +861,56 @@ Proof.
   intros. red in H0. inv H; constructor; auto; intros.
 - rewrite H0; auto. unfold mreg_within_bounds in H. tauto.
 - rewrite <- agree_incoming0 by auto. apply H0. congruence.
+Qed.
+
+
+Definition agree_unused_rs (rs0 rs :regset) : Prop :=
+  forall r, ~(mreg_within_bounds b r) -> rs0 r = rs r.
+
+
+Lemma agree_unused_rs_set_reg : forall rs rs0 r v,
+    agree_unused_rs rs rs0 ->
+    mreg_within_bounds b r ->
+    agree_unused_rs (Regmap.set r v rs) rs0.
+Proof.
+  intros. red. intros. red in H.
+  rewrite Regmap.gso. auto. red. intuition congruence.
+Qed.
+
+Lemma agree_unused_rs_undef_regs_1:
+  forall rs0 regs rs ,
+  agree_unused_rs rs rs0 ->
+  (forall r, In r regs -> mreg_within_bounds b r) ->
+  agree_unused_rs (undef_regs regs rs) rs0.
+Proof.
+  induction regs; simpl; intros.
+  auto.
+  apply agree_unused_rs_set_reg; auto.
+Qed.
+
+Lemma agree_unused_rs_undef_regs:
+  forall rs0 regs rs,
+    agree_unused_rs rs rs0 ->
+    existsb is_callee_save regs = false ->
+  agree_unused_rs (undef_regs regs rs) rs0.
+Proof.
+  intros. eapply agree_unused_rs_undef_regs_1; eauto.
+  intros. destruct (is_callee_save r) eqn:CS; auto.
+  assert (existsb is_callee_save regs = true).
+  { apply existsb_exists. exists r; auto. }
+  congruence. congruence.
+Qed.
+
+Lemma agree_unused_rs_set_res:
+  forall rs0 res v rs,
+  agree_unused_rs rs rs0 ->
+  (forall r, In r (params_of_builtin_res res) -> mreg_within_bounds b r) ->
+  agree_unused_rs (set_res res v rs) rs0.
+Proof.
+  induction res; simpl; intros.
+- eapply agree_unused_rs_set_reg; eauto.
+- auto.
+- apply IHres2; auto using in_or_app.
 Qed.
 
 (** ** Properties of destroyed registers. *)
@@ -930,6 +1008,12 @@ Qed.
   the register save areas of the current frame do contain the
   values of the callee-save registers used by the function. *)
 
+Lemma reg_type_64 : forall r, mreg_type r = Tany64.
+Proof. intros. destruct r; eauto. Qed.
+
+Lemma reg_well_type : forall rs r, Val.has_type (rs r) (mreg_type r).
+Proof. intros. rewrite reg_type_64. destruct (rs r); constructor. Qed.
+
 Section SAVE_CALLEE_SAVE.
 
 Variable j: meminj.
@@ -937,6 +1021,7 @@ Variable cs: list stackframe.
 Variable vf: val.
 Variable sp: block.
 Variable ls: locset.
+Variable rs0: regset.
 
 Hypothesis ls_temp_undef:
   forall ty r, In r (destroyed_by_setstack ty) -> ls (R r) = Vundef.
@@ -949,23 +1034,26 @@ Lemma save_callee_save_rec_correct:
   (forall r, In r l -> is_callee_save r = true) ->
   m |= range sp pos (size_callee_save_area_rec l pos) ** P ->
   agree_regs j ls rs ->
+  (forall r, In r l -> rs0 r = rs r) ->
   exists rs', exists m',
      star step tge
         (State cs vf (Vptr sp Ptrofs.zero) (save_callee_save_rec l pos k) rs m)
      E0 (State cs vf (Vptr sp Ptrofs.zero) k rs' m')
-  /\ m' |= contains_callee_saves j sp pos l ls ** P
+  /\ m' |= contains_callee_saves j sp pos l ls rs0 ** P
   /\ (forall ofs k p, Mem.perm m sp ofs k p -> Mem.perm m' sp ofs k p)
   /\ agree_regs j ls rs'
+  /\ agree_unused_rs rs' rs
   /\ Mem.support m = Mem.support m'
   /\ Mem.unchanged_on (fun b ofs => b <> sp) m m'.
 Proof.
 Local Opaque mreg_type.
-  induction l as [ | r l]; simpl; intros until P; intros CS SEP AG.
+  induction l as [ | r l]; simpl; intros until P; intros CS SEP AG RSS.
 - exists rs, m.
   split. apply star_refl.
   split. rewrite sep_pure; split; auto. eapply sep_drop; eauto.
   split. auto.
   split; auto.
+  split. red. intros. eauto.
   split; eauto with mem.
 - set (ty := mreg_type r) in *.
   set (sz := AST.typesize ty) in *.
@@ -981,10 +1069,10 @@ Local Opaque mreg_type.
   apply range_split with (mid := pos1 + sz) in SEP; [ | lia ].
   unfold sz at 1 in SEP. rewrite <- size_type_chunk in SEP.
   apply range_contains in SEP; auto.
-  exploit (contains_set_stack (fun v' => Val.inject j (ls (R r)) v') (rs r)).
-  eexact SEP. 
+  exploit (contains_set_stack (fun v' => Val.inject j (ls (R r)) v' /\ rs0 r = v') (rs r)).
+  eexact SEP. split.
   apply load_result_inject; [auto|apply wt_ls].
-  (* erewrite Val.load_result_same. eauto. unfold ty. apply reg_well_type. *)
+  erewrite Val.load_result_same. eauto. unfold ty. apply reg_well_type.
   clear SEP; intros (m1 & STORE & SEP).
   set (rs1 := undef_regs (destroyed_by_setstack ty) rs).
   assert (AG1: agree_regs j ls rs1).
@@ -1000,23 +1088,21 @@ Local Opaque mreg_type.
     eapply existsb_exists. exists r0. split. auto. eauto. congruence.
   }
   rewrite sep_swap in SEP.
-  exploit (IHl (pos1 + sz) rs1 m1); eauto. 
-  (* rewrite RSS. *) (* eauto. right. auto. *)
-  intros (rs2 & m2 & A & B & C & D & E & F).
+  exploit (IHl (pos1 + sz) rs1 m1); eauto. intros. rewrite RSS. eauto. right. auto.
+  intros (rs2 & m2 & A & B & C & D & E & F & G).
   exists rs2, m2.
   split. eapply star_left; eauto. constructor. exact STORE. auto. traceEq.
   split. rewrite sep_assoc, sep_swap. exact B.
   split. intros. apply C. unfold store_stack in STORE; simpl in STORE. eapply Mem.perm_store_1; eauto.
   split.  eauto. split. 
-  (* assert (agree_unused_rs rs1 rs). unfold rs1. *)
-  (* eapply agree_unused_rs_undef_regs; eauto. red. intros. eauto. *)
-  (* eapply  destroyed_by_setstack_caller_save. *)
-  (* red. intros. rewrite E; eauto. split. *)
+  assert (agree_unused_rs rs1 rs). unfold rs1.
+  eapply agree_unused_rs_undef_regs; eauto. red. intros. eauto.
+  eapply  destroyed_by_setstack_caller_save.
+  red. intros. rewrite E; eauto. split.
   erewrite Mem.support_storev. 2: eauto. auto.
   eapply Mem.unchanged_on_trans; eauto. eapply Mem.store_unchanged_on.
   apply STORE. eauto.
 Qed.
-
 
 End SAVE_CALLEE_SAVE.
 
@@ -1066,20 +1152,27 @@ Lemma save_callee_save_correct:
      star step tge
         (State cs fb (Vptr sp Ptrofs.zero) (save_callee_save fe k) rs1 m)
      E0 (State cs fb (Vptr sp Ptrofs.zero) k rs' m')
-  /\ m' |= contains_callee_saves j sp fe.(fe_ofs_callee_save) b.(used_callee_save) ls0 ** P
+  /\ m' |= contains_callee_saves j sp fe.(fe_ofs_callee_save) b.(used_callee_save) ls0 rs ** P
   /\ (forall ofs k p, Mem.perm m sp ofs k p -> Mem.perm m' sp ofs k p)
   /\ agree_regs j ls1 rs'
+  /\ agree_unused_rs rs' rs
   /\ Mem.support m = Mem.support m'
   /\ Mem.unchanged_on (fun b ofs => b <> sp) m m'.
 Proof.
   intros until P; intros SEP TY AGCS AG; intros ls1 rs1.
-  exploit (save_callee_save_rec_correct j cs fb sp ls1).
+  exploit (save_callee_save_rec_correct j cs fb sp ls1 rs).
 - intros. unfold ls1. apply LTL_undef_regs_same. eapply destroyed_by_setstack_function_entry; eauto.
 - intros. unfold ls1. apply undef_regs_type. apply TY.
 - exact b.(used_callee_save_prop).
 - eexact SEP.
 - instantiate (1 := rs1). apply agree_regs_undef_regs. apply agree_regs_call_regs. auto.
-- clear SEP. intros (rs' & m' & EXEC & SEP & PERMS & AG' & SUP & UNC ).
+- intros. unfold rs1. rewrite undef_regs_other. auto. intro.
+  generalize (destroyed_at_function_entry_caller_save).
+  intro. red in H1.
+  assert ( existsb is_callee_save (destroyed_at_function_entry) = true).
+  eapply existsb_exists. exists r. split. auto. 
+  eapply used_callee_save_prop; eauto. congruence.
+- clear SEP. intros (rs' & m' & EXEC & SEP & PERMS & AG' & AG'' & TE').
   exists rs', m'.
   split. eexact EXEC.
   split. rewrite (contains_callee_saves_exten j sp ls0 ls1). exact SEP.
@@ -1092,12 +1185,11 @@ Proof.
     assert (existsb is_callee_save destroyed_at_function_entry = true).
     { apply existsb_exists. exists r; auto. }
     congruence.
-    (* reflexivity. *)
+    reflexivity.
     split. exact PERMS. split. exact AG'. split.
-    (* assert (agree_unused_rs rs1 rs). unfold rs1. eapply agree_unused_rs_undef_regs. red. intros. eauto. *)
-    eauto. eauto.
-    (* eapply destroyed_at_function_entry_caller_save. red. intros. erewrite AG''; eauto. *)
-    (* exact TE'. *)
+    assert (agree_unused_rs rs1 rs). unfold rs1. eapply agree_unused_rs_undef_regs. red. intros. eauto.
+    eapply destroyed_at_function_entry_caller_save. red. intros. erewrite AG''; eauto.
+    exact TE'.
 Qed.
 
 (** As a corollary of the previous lemmas, we obtain the following
@@ -1105,6 +1197,9 @@ Qed.
   (allocation of the frame + saving of the link and return address +
   saving of the used callee-save registers). *)
 
+(* Lemma fe_size_eq: Linear.fn_stacksize f = fe_size fe. *)
+(* Proof. *)
+(*   unfold fe. unfold b. simpl. *)
 
 Lemma function_prologue_correct:
   forall j ls ls0 ls1 rs rs1 m1 m1' m2 sp parent ra cs fb k P
@@ -1127,7 +1222,8 @@ Lemma function_prologue_correct:
       E0 (State cs fb (Vptr sp' Ptrofs.zero) k rs' m5')
   /\ agree_regs j' ls1 rs'
   /\ agree_locs ls1 ls0
-  /\ m5' |= frame_contents j' sp' ls1 ls0 parent ra ** minjection j' m2 ** globalenv_inject se tse j' m2 ** P
+  /\ agree_unused_rs rs' rs
+  /\ m5' |= frame_contents j' sp' ls1 ls0 rs parent ra ** minjection j' m2 ** globalenv_inject se tse j' m2 ** P
   /\ j' sp = Some(sp', fe.(fe_stack_data))
   /\ inject_incr j j'
   /\ inject_separated j j' m1 m1'
@@ -1180,7 +1276,7 @@ Local Opaque b fe.
   apply agree_regs_inject_incr with j; auto.
   replace (LTL.undef_regs destroyed_at_function_entry (call_regs ls)) with ls1 by auto.
   replace (undef_regs destroyed_at_function_entry rs) with rs1 by auto.
-  clear SEP; intros (rs2 & m5' & SAVE_CS & SEP & PERMS & AGREGS' & SUP & UNC).
+  clear SEP; intros (rs2 & m5' & SAVE_CS & SEP & PERMS & AGREGS' & AGREGS''& TE' & UNC).
   rewrite sep_swap5 in SEP.
   (* Materializing the Local and Outgoing locations *)
   exploit (initial_locations j'). eexact SEP. tauto.
@@ -1194,7 +1290,7 @@ Local Opaque b fe.
   clear SEP; intros SEP.
   rewrite sep_swap in SEP.
   (* Now we frame this *)
-  assert (SEPFINAL: m5' |= frame_contents j' sp' ls1 ls0 parent ra ** minjection j' m2 ** globalenv_inject se tse j' m2 ** P).
+  assert (SEPFINAL: m5' |= frame_contents j' sp' ls1 ls0 rs parent ra ** minjection j' m2 ** globalenv_inject se tse j' m2 ** P).
   { eapply frame_mconj. eexact SEPCONJ.
     rewrite chunk_of_Tptr in SEP.
     unfold frame_contents_1; rewrite ! sep_assoc. exact SEP.
@@ -1231,7 +1327,7 @@ Local Opaque b fe.
     - red. intros. inv UNC2. eapply unchanged_on_perm; eauto.
       intros. simpl. intro. subst. 
       eapply Mem.fresh_block_alloc; eauto.
-    - split. rewrite <- SUP. rewrite <- SUP34. rewrite <- SUP23.
+    - split. rewrite <- TE'. rewrite <- SUP34. rewrite <- SUP23.
       inv H11. eauto.
       eapply mem_unchanged_on_trans_implies_valid. 2: eauto.
       eauto with mem. intros. intro. subst.
@@ -1254,11 +1350,10 @@ Local Opaque b fe.
     unfold mreg_within_bounds in H0; tauto.
     unfold call_regs. apply AGARGS. apply incoming_slot_in_parameters; auto.
   split. eauto.
-  (* split. exact SEPFINAL. *)
+  split. exact SEPFINAL.
   split. exact SAME.
   split. exact INCR. split. exact INJSEP. auto.
 Qed.
-
 
 (** The following lemmas show the correctness of the register reloading
   code generated by [reload_callee_save]: after this code has executed,
@@ -1272,14 +1367,16 @@ Variable cs: list stackframe.
 Variable fb: val.
 Variable sp: block.
 Variable ls0: locset.
+Variable rs0: regset.
 Variable m: mem.
 
 Definition agree_unused (ls0: locset) (rs: regset) : Prop :=
   forall r, ~(mreg_within_bounds b r) -> Val.inject j (ls0 (R r)) (rs r).
 
+
 Lemma restore_callee_save_rec_correct:
   forall l ofs rs k,
-  m |= contains_callee_saves j sp ofs l ls0 ->
+  m |= contains_callee_saves j sp ofs l ls0 rs0 ->
   agree_unused ls0 rs ->
   (forall r, In r l -> mreg_within_bounds b r) ->
   exists rs',
@@ -1287,6 +1384,7 @@ Lemma restore_callee_save_rec_correct:
       (State cs fb (Vptr sp Ptrofs.zero) (restore_callee_save_rec l ofs k) rs m)
    E0 (State cs fb (Vptr sp Ptrofs.zero) k rs' m)
   /\ (forall r, In r l -> Val.inject j (ls0 (R r)) (rs' r))
+  /\ (forall r, In r l -> rs' r = rs0 r)
   /\ (forall r, ~(In r l) -> rs' r = rs r)
   /\ agree_unused ls0 rs'.
 Proof.
@@ -1303,36 +1401,44 @@ Local Opaque mreg_type.
   assert (BOUND: mreg_within_bounds b r) by eauto.
   exploit contains_get_stack.
     eapply sep_proj1; eassumption.
-  intros (v & LOAD & SPEC).
+  intros (v & LOAD & SPEC1 & SPEC2).
   exploit (IHl (ofs1 + sz) (rs#r <- v)).
     eapply sep_proj2; eassumption.
     red; intros. rewrite Regmap.gso. auto. intuition congruence.
     eauto.
-  intros (rs' & A & B & C & D).
+  intros (rs' & A & B & C & D & E).
   exists rs'.
   split. eapply star_step; eauto.
     econstructor. exact LOAD. traceEq.
   split. intros.
     destruct (In_dec mreg_eq r0 l). auto.
     assert (r = r0) by tauto. subst r0.
-    rewrite C by auto. rewrite Regmap.gss. exact SPEC.
+    rewrite D by auto. rewrite Regmap.gss. exact SPEC1.
   split. intros.
-    rewrite C by tauto. apply Regmap.gso. intuition auto.
-  exact D.
+    destruct (In_dec mreg_eq r0 l). auto.
+    assert (r = r0) by tauto. subst r0.
+    rewrite D by auto. rewrite Regmap.gss. eauto.
+  split. intros.
+    rewrite D by tauto. apply Regmap.gso. intuition auto.
+  exact E.
 Qed.
 
 End RESTORE_CALLEE_SAVE.
 
+
 Lemma restore_callee_save_correct:
-  forall m j sp ls ls0 pa ra P rs k cs fb,
-  m |= frame_contents j sp ls ls0 pa ra ** P ->
+  forall m j sp ls ls0 rs0 pa ra P rs k cs fb,
+  m |= frame_contents j sp ls ls0 rs0 pa ra ** P ->
   agree_unused j ls0 rs ->
+  agree_unused_rs rs0 rs ->
   exists rs',
     star step tge
        (State cs fb (Vptr sp Ptrofs.zero) (restore_callee_save fe k) rs m)
     E0 (State cs fb (Vptr sp Ptrofs.zero) k rs' m)
   /\ (forall r,
-        is_callee_save r = true -> Val.inject j (ls0 (R r)) (rs' r))
+         is_callee_save r = true -> Val.inject j (ls0 (R r)) (rs' r))
+  /\ (forall r,
+         is_callee_save r = true -> rs0 r = rs' r)
   /\ (forall r,
         is_callee_save r = false -> rs' r = rs r).
 Proof.
@@ -1341,14 +1447,18 @@ Proof.
   apply mconj_proj1 in H. rewrite ! sep_assoc in H. apply sep_pick5 in H.
   exploit restore_callee_save_rec_correct; eauto.
   intros; unfold mreg_within_bounds; auto.
-  intros (rs' & A & B & C & D).
+  intros (rs' & A & B & C & D & E).
   exists rs'.
   split. eexact A.
   split; intros.
   destruct (In_dec mreg_eq r (used_callee_save b)).
   apply B; auto.
-  rewrite C by auto. apply H0. unfold mreg_within_bounds; tauto.
-  apply C. red; intros. apply (used_callee_save_prop b) in H2. congruence.
+  rewrite D by auto. apply H0. unfold mreg_within_bounds; tauto.
+  split; intros.
+  destruct (In_dec mreg_eq r (used_callee_save b)).
+  rewrite C; eauto.
+  rewrite D by auto. apply H1. unfold mreg_within_bounds; tauto.
+  apply D. red; intros. apply (used_callee_save_prop b) in H3. congruence.
 Qed.
 
 (** As a corollary, we obtain the following correctness result for
@@ -1356,11 +1466,13 @@ Qed.
   registers + reloading of the link and return address + freeing
   of the frame). *)
 
+
 Lemma function_epilogue_correct:
-  forall m' j sp' ls ls0 pa ra P m rs sp m1 k cs fb,
-  m' |= frame_contents j sp' ls ls0 pa ra ** minjection j m ** P ->
+  forall m' j sp' ls ls0 rs0 pa ra P m rs sp m1 k cs fb,
+  m' |= frame_contents j sp' ls ls0 rs0 pa ra ** minjection j m ** P -> 
   agree_regs j ls rs ->
   agree_locs ls ls0 ->
+  agree_unused_rs rs rs0 ->
   j sp = Some(sp', fe.(fe_stack_data)) ->
   Mem.free m sp 0 f.(Linear.fn_stacksize) = Some m1 ->
   exists rs1, exists m1',
@@ -1372,22 +1484,24 @@ Lemma function_epilogue_correct:
     E0 (State cs fb (Vptr sp' Ptrofs.zero) k rs1 m')
   /\ agree_regs j (return_regs ls0 ls) rs1
   /\ agree_callee_save (return_regs ls0 ls) ls0
+  /\ (forall r, is_callee_save r = true -> rs0 r = rs1 r)
   /\ m1' |= minjection j m1 ** P.
 Proof.
-  intros until fb; intros SEP AGR AGL INJ FREE.
+  intros until fb; intros SEP AGR AGL AGRS INJ FREE.
   (* Can free *)
   exploit free_parallel_rule.
-    rewrite <- sep_assoc. eapply mconj_proj2. eexact SEP.
-    eexact FREE.
+    rewrite <- sep_assoc. eapply mconj_proj2. eexact SEP. eauto.
+    (* eexact FREE. *)
     eexact INJ.
     auto. rewrite Z.max_comm; reflexivity.
   intros (m1' & FREE' & SEP').
   (* Reloading the callee-save registers *)
   exploit restore_callee_save_correct.
-    eexact SEP.
-    instantiate (1 := rs).
-    red; intros. destruct AGL. rewrite <- agree_unused_reg0 by auto. apply AGR.
-  intros (rs' & LOAD_CS & CS & NCS).
+  eexact SEP.
+  instantiate (1 := rs).
+  red; intros. destruct AGL. rewrite <- agree_unused_reg0 by auto. apply AGR.
+  red. intros. exploit AGRS; eauto.
+  intros (rs' & LOAD_CS & CS & SAVE & NCS).
   (* Reloading the back link and return address *)
   unfold frame_contents in SEP; apply mconj_proj1 in SEP.
   unfold frame_contents_1 in SEP; rewrite ! sep_assoc in SEP.
@@ -1406,8 +1520,8 @@ Proof.
     apply CS; auto.
     rewrite NCS by auto. apply AGR.
   split. red; unfold return_regs; intros.
-    destruct l. rewrite H; auto. destruct sl; auto; contradiction. 
-  assumption.
+  destruct l. rewrite H; auto. destruct sl; auto; contradiction.
+  split. assumption. assumption.
 Qed.
 
 End FRAME_PROPERTIES.
@@ -1421,15 +1535,22 @@ Variable w : cc_stacking_world injp.
 (** This is the memory assertion that captures the contents of the stack frames
   mentioned in the call stacks. *)
 
-Fixpoint stack_contents (j: meminj) (cs: list Linear.stackframe) (cs': list Mach.stackframe) : massert :=
-  match cs, cs' with
-  | Linear.Stackbase ls :: nil, Mach.Stackbase _ ra :: nil =>
+
+Definition parent_rs (s: list regset)  :=
+  match s with
+  | nil => stk_rs2 w
+  | hd :: tl => hd
+  end.
+
+Fixpoint stack_contents (j: meminj) (cs: list Linear.stackframe) (cs': list Mach.stackframe) (lrs' : list regset): massert :=
+  match cs, cs', lrs' with
+  | Linear.Stackbase ls :: nil, Mach.Stackbase _ ra :: nil, nil =>
       contains_init_args (stk_sg w) j ls (stk_m2 w) (stk_sp2 w)
 (*      **  contains_init_sp_ra (stk_sg w) (stk_fsz2 w) (stk_m2 w) (stk_sp2 w) *)
-  | Linear.Stackframe f _ ls c :: cs, Mach.Stackframe fb (Vptr sp' _) ra c' :: cs' =>
-      frame_contents f j sp' ls (parent_locset cs) (parent_sp cs') (parent_ra cs')
-      ** stack_contents j cs cs'
-  | _, _ => pure False
+  | Linear.Stackframe f _ ls c :: cs, Mach.Stackframe fb (Vptr sp' _) ra c' :: cs', hd :: tl =>
+      frame_contents f j sp' ls (parent_locset cs) (parent_rs tl) (parent_sp cs') (parent_ra cs')
+      ** stack_contents j cs cs' tl
+  | _, _, _ => pure False
   end.
 
 (** [match_stacks] captures additional properties (not related to memory)
@@ -1446,7 +1567,7 @@ Definition init_m2' := stk_m2 w.
 Definition init_sp2 := stk_sp2 w.
 
 Inductive match_stacks (j: meminj):
-       list Linear.stackframe -> list stackframe -> signature -> Prop :=
+       list Linear.stackframe -> list stackframe -> list regset -> signature -> Prop :=
   | match_stacks_base: forall ra sg
         (TY_SP: Val.has_type (stk_sp2 w) Tptr)
         (TY_RA: Val.has_type ra Tptr),
@@ -1455,13 +1576,14 @@ Inductive match_stacks (j: meminj):
       (* injw_sup_r (stk_w w) = (Mem.support (stk_m2 w)) -> *)
       init_m2 = init_m2' ->
       (forall b1 b2 delta, init_j b1 = None -> j b1 = Some (b2, delta) ->
-                      ~ sup_In b1 (Mem.support (init_m1)) /\
-                        ~ sup_In b2 (Mem.support (init_m2)))  ->
+         ~ sup_In b1 (Mem.support (init_m1)) /\
+         ~ sup_In b2 (Mem.support (init_m2)))  ->
       match_stacks j
                    (Linear.Stackbase (initial_regs (stk_sg w) (stk_ls1 w)) :: nil)
                    (Stackbase (stk_sp2 w) ra :: nil)
+                   nil
                    sg
-  | match_stacks_cons: forall f sp ls c cs fb sp' ra c' cs' sg trf
+  | match_stacks_cons: forall f sp ls c cs fb sp' ra c' cs' sg trf lrs' rs
         (TAIL: is_tail c (Linear.fn_code f))
         (FINDF: Genv.find_funct tge fb = Some (Internal trf))
         (TRF: transf_function f = OK trf)
@@ -1469,17 +1591,19 @@ Inductive match_stacks (j: meminj):
         (INJ: j sp = Some(sp', (fe_stack_data (make_env (function_bounds f)))))
         (NEWSP: ~ Mem.valid_block init_m1 sp /\ ~ Mem.valid_block init_m2 sp')
         (TY_RA: Val.has_type ra Tptr)
+        (RAN: ra <> Vundef)
         (AGL: agree_locs f ls (parent_locset cs))
+        (AGRS: agree_unused_rs f rs (parent_rs lrs'))
         (ARGS: forall ofs ty,
            In (S Outgoing ofs ty) (regs_of_rpairs (loc_arguments sg)) ->
            slot_within_bounds (function_bounds f) Outgoing ofs ty)
         (SZA: size_arguments sg <= bound_outgoing (function_bounds f))
-        (STK: match_stacks j cs cs' (Linear.fn_sig f)),
+        (STK: match_stacks j cs cs' lrs' (Linear.fn_sig f)),
       match_stacks j
                    (Linear.Stackframe f (Vptr sp Ptrofs.zero) ls c :: cs)
                    (Stackframe fb (Vptr sp' Ptrofs.zero) ra c' :: cs')
+                   (rs :: lrs')
                    sg.
-
 (** Invariance with respect to change of memory injection. *)
 
 Lemma contains_init_args_incr:
@@ -1494,14 +1618,15 @@ Proof.
   intros ofs ty REG. edestruct ARGS as (? & ? & ?); eauto.
 Qed.
 
+
 Lemma stack_contents_change_meminj:
   forall m j j', inject_incr j j' ->
-  forall cs cs' P,
-  m |= stack_contents j cs cs' ** P ->
-  m |= stack_contents j' cs cs' ** P.
+  forall cs cs' lrs P,
+  m |= stack_contents j cs cs' lrs ** P ->
+  m |= stack_contents j' cs cs' lrs ** P.
 Proof.
 Local Opaque sepconj.
-  induction cs as [ | [] cs]; destruct cs' as [ | [] cs']; simpl; intros; auto.
+  induction cs as [ | [] cs]; destruct cs' as [ | [] cs']; destruct lrs; simpl; intros; auto.
 - destruct sp0; auto.
   rewrite sep_assoc in *.
   apply frame_contents_incr with (j := j); auto.
@@ -1516,9 +1641,9 @@ Lemma match_stacks_change_meminj:
   inject_separated j j' m m' ->
   Mem.sup_include (Mem.support init_m1) (Mem.support m) ->
   Mem.sup_include (Mem.support init_m2) (Mem.support m') ->
-  forall cs cs' sg,
-  match_stacks j cs cs' sg ->
-  match_stacks j' cs cs' sg.
+  forall cs cs' lrs sg,
+  match_stacks j cs cs' lrs sg ->
+  match_stacks j' cs cs' lrs sg.
 Proof.
   induction 5; intros.
 - constructor; auto.
@@ -1528,10 +1653,10 @@ Proof.
     * edestruct H0; eauto. unfold Mem.valid_block in *. split; eauto.
 - econstructor; eauto.
 Qed.
-  
-Lemma stack_contents_support m j cs cs' sg:
-  m |= stack_contents j cs cs' ->
-  match_stacks j cs cs' sg ->
+
+Lemma stack_contents_support m j cs cs' lrs sg:
+  m |= stack_contents j cs cs' lrs ->
+  match_stacks j cs cs' lrs sg ->
   Mem.sup_include (Mem.support init_m2) (Mem.support m).
 Proof.
   induction 2.
@@ -1542,10 +1667,10 @@ Qed.
 (** Invariance with respect to change of signature. *)
 
 Lemma match_stacks_change_sig:
-  forall sg1 j cs cs' sg,
-  match_stacks j cs cs' sg ->
+  forall sg1 j cs cs' lrs sg,
+  match_stacks j cs cs' lrs sg ->
   tailcall_possible sg1 ->
-  match_stacks j cs cs' sg1.
+  match_stacks j cs cs' lrs sg1.
 Proof.
   induction 1; intros.
   econstructor; eauto.
@@ -1558,16 +1683,16 @@ Qed.
 (** Typing properties of [match_stacks]. *)
 
 Lemma match_stacks_type_sp:
-  forall j cs cs' sg,
-  match_stacks j cs cs' sg ->
+  forall j cs cs' lrs sg,
+  match_stacks j cs cs' lrs sg ->
   Val.has_type (parent_sp cs') Tptr.
 Proof.
   destruct 1; auto; constructor.
 Qed.
 
 Lemma match_stacks_type_retaddr:
-  forall j cs cs' sg,
-  match_stacks j cs cs' sg ->
+  forall j cs cs' lrs sg,
+  match_stacks j cs cs' lrs sg ->
   Val.has_type (parent_ra cs') Tptr.
 Proof.
   induction 1; unfold parent_ra; auto.
@@ -1575,10 +1700,11 @@ Qed.
 
 (** Accessing the parent's outgoing locations *)
 
-Lemma load_stack_arg m j cs cs' sg ty ofs:
+
+Lemma load_stack_arg m j cs cs' lrs sg ty ofs:
   In (S Outgoing ofs ty) (regs_of_rpairs (loc_arguments sg)) ->
-  match_stacks j cs cs' sg ->
-  m |= stack_contents j cs cs' ->
+  match_stacks j cs cs' lrs sg ->
+  m |= stack_contents j cs cs' lrs ->
   exists v,
      load_stack m (parent_sp cs') ty (Ptrofs.repr (offset_arg ofs)) = Some v
   /\ Val.inject j (parent_locset cs (S Outgoing ofs ty)) v.
@@ -1593,9 +1719,9 @@ Proof.
     rewrite zle_true by lia. rewrite pred_dec_true by auto. reflexivity.
 Qed.
 
-Lemma match_stacks_range_perm_args m j cs cs' sg sb sofs:
-  match_stacks j cs cs' sg ->
-  m |= stack_contents j cs cs' ->
+Lemma match_stacks_range_perm_args m j cs cs' lrs sg sb sofs:
+  match_stacks j cs cs' lrs sg ->
+  m |= stack_contents j cs cs' lrs ->
   parent_sp cs' = Vptr sb sofs ->
   Mem.range_perm m sb (offset_sarg sofs 0) (offset_sarg sofs (size_arguments sg)) Cur Freeable.
 Proof.
@@ -1616,9 +1742,9 @@ Proof.
     + unfold Ptrofs.max_unsigned. extlia.
 Qed.
 
-Lemma match_stacks_args_fit m j cs cs' sg ofs sb sofs:
-  match_stacks j cs cs' sg ->
-  m |= stack_contents j cs cs' ->
+Lemma match_stacks_args_fit m j cs cs' lrs sg ofs sb sofs:
+  match_stacks j cs cs' lrs sg ->
+  m |= stack_contents j cs cs' lrs ->
   parent_sp cs' = Vptr sb sofs ->
   0 <= ofs < size_arguments sg ->
   offset_fits sofs ofs.
@@ -1635,9 +1761,9 @@ Proof.
       unfold Ptrofs.max_unsigned; extlia.
 Qed.
 
-Lemma match_stacks_init_args j cs cs' sg m P:
-  match_stacks j cs cs' sg ->
-  m |= stack_contents j cs cs' ** P ->
+Lemma match_stacks_init_args j cs cs' lrs sg m P:
+  match_stacks j cs cs' lrs sg ->
+  m |= stack_contents j cs cs' lrs ** P ->
   m |= contains_init_args sg j (parent_locset cs) m (parent_sp cs') ** P.
 Proof.
   intros MS SEP. split.
@@ -1842,16 +1968,17 @@ Section EXTERNAL_ARGUMENTS.
 Variable j: meminj.
 Variable cs: list Linear.stackframe.
 Variable cs': list stackframe.
+Variable lrs: list regset.
 Variable sg: signature.
 Variables bound bound': block.
-Hypothesis MS: match_stacks j cs cs' sg.
+Hypothesis MS: match_stacks j cs cs' lrs sg.
 Variable ls: locset.
 Variable rs: regset.
 Hypothesis AGR: agree_regs j ls rs.
 Hypothesis AGCS: agree_callee_save ls (parent_locset cs).
 Hypothesis AGARGS: agree_outgoing_arguments sg ls (parent_locset cs).
 Variable m': mem.
-Hypothesis SEP: m' |= stack_contents j cs cs'.
+Hypothesis SEP: m' |= stack_contents j cs cs' lrs.
 
 Lemma transl_external_argument:
   forall l,
@@ -1920,12 +2047,13 @@ Hypothesis TRANSF_F: transf_function f = OK tf.
 Variable j: meminj.
 Variables m m': mem.
 Variables ls ls0: locset.
-Variable rs: regset.
+Variable rs0 rs: regset.
 Variables sp sp': block.
 Variables parent retaddr: val.
 Hypothesis INJ: j sp = Some(sp', fe.(fe_stack_data)).
 Hypothesis AGR: agree_regs j ls rs.
-Hypothesis SEP: m' |= frame_contents f j sp' ls ls0 parent retaddr ** minjection j m ** globalenv_inject se tse j m.
+Hypothesis SEP: m' |= frame_contents f j sp' ls ls0 rs0 parent retaddr ** minjection j m ** globalenv_inject se tse j m.
+
 
 Lemma transl_builtin_arg_correct:
   forall a v,
@@ -2080,18 +2208,19 @@ Qed.
 
 Inductive match_states: Linear.state -> Mach.state -> Prop :=
   | match_states_intro:
-      forall cs f sp c ls m cs' fb sp' rs m' j tf
+      forall cs f sp c ls m cs' fb sp' rs m' j tf lrs
         (NB: Mem.sup_include (Mem.support init_m1) (Mem.support m))
-        (STACKS: match_stacks j cs cs' f.(Linear.fn_sig))
+        (STACKS: match_stacks j cs cs' lrs f.(Linear.fn_sig))
         (TRANSL: transf_function f = OK tf)
         (FIND: Genv.find_funct tge fb = Some (Internal tf))
         (AGREGS: agree_regs j ls rs)
+        (AGLOCST: agree_unused_rs f rs (parent_rs lrs))
         (AGLOCS: agree_locs f ls (parent_locset cs))
         (INJSP: j sp = Some(sp', fe_stack_data (make_env (function_bounds f))))
         (NEWSP: ~ Mem.valid_block init_m1 sp /\ ~ Mem.valid_block init_m2 sp')
         (TAIL: is_tail c (Linear.fn_code f))
-        (SEP: m' |= frame_contents f j sp' ls (parent_locset cs) (parent_sp cs') (parent_ra cs')
-                 ** stack_contents j cs cs'
+        (SEP: m' |= frame_contents f j sp' ls (parent_locset cs) (parent_rs lrs) (parent_sp cs') (parent_ra cs')
+                 ** stack_contents j cs cs' lrs
                  ** minjection j m
                  ** globalenv_inject se tse j m)
         (Hm: Mem.inject j m m')
@@ -2099,13 +2228,14 @@ Inductive match_states: Linear.state -> Mach.state -> Prop :=
       match_states (Linear.State cs f (Vptr sp Ptrofs.zero) c ls m)
                    (Mach.State cs' fb (Vptr sp' Ptrofs.zero) (transl_code (make_env (function_bounds f)) c) rs m')
   | match_states_call:
-      forall cs vf f ls m cs' vf' rs m' j
+      forall cs vf f ls m cs' vf' rs m' j lrs
         (NB: Mem.sup_include (Mem.support init_m1) (Mem.support m))
-        (STACKS: match_stacks j cs cs' (Linear.funsig f))
+        (STACKS: match_stacks j cs cs' lrs (Linear.funsig f))
         (FIND: Genv.find_funct ge vf = Some f)
         (FINJ: Val.inject j vf vf')
         (AGREGS: agree_regs j ls rs)
-        (SEP: m' |= stack_contents j cs cs'
+        (TRS: forall r, is_callee_save r = true -> rs r = parent_rs lrs r) (*This could be rs = parent_rs lrs if we do not consider tailcall*)
+        (SEP: m' |= stack_contents j cs cs' lrs
                  ** minjection j m
                  ** globalenv_inject se tse j m)
         (Hm: Mem.inject j m m')
@@ -2113,14 +2243,15 @@ Inductive match_states: Linear.state -> Mach.state -> Prop :=
       match_states (Linear.Callstate cs vf ls m)
                    (Mach.Callstate cs' vf' rs m')
   | match_states_return:
-      forall cs ls m cs' rs m' j sg
+      forall cs ls m cs' rs m' j sg lrs
         (NB: Mem.sup_include (Mem.support init_m1) (Mem.support m))
-        (STACKS: match_stacks j cs cs' sg)
+        (STACKS: match_stacks j cs cs' lrs sg)
         (AGREGS: agree_regs j ls rs)
-        (SEP: m' |= stack_contents j cs cs'
+        (CALLEESAVE: forall r, is_callee_save r = true -> rs r = (parent_rs lrs) r)
+        (SEP: m' |= stack_contents j cs cs' lrs
                  ** minjection j m
                  ** globalenv_inject se tse j m)
-      (Hm: Mem.inject j m m')
+        (Hm: Mem.inject j m m')
       (ACC: injp_acc init_wj (injpw j m m' Hm)),
       match_states (Linear.Returnstate cs ls m)
                   (Mach.Returnstate cs' rs m').
@@ -2147,6 +2278,7 @@ Proof.
   apply plus_one. apply exec_Mgetstack. exact A.
   econstructor; eauto with coqlib.
   apply agree_regs_set_reg; auto.
+  apply agree_unused_rs_set_reg; auto.
   apply agree_locs_set_reg; auto.
 + (* Lgetstack, incoming *)
   unfold slot_valid in SV. InvBooleans.
@@ -2159,6 +2291,9 @@ Proof.
   econstructor; eauto with coqlib.
   apply agree_regs_set_reg. apply agree_regs_set_reg. auto. auto.
   erewrite agree_incoming by eauto. exact B.
+  apply agree_unused_rs_set_reg; eauto.
+  apply agree_unused_rs_set_reg; eauto.
+  eapply  caller_save_reg_within_bounds; eauto.
   apply agree_locs_set_reg; auto. apply agree_locs_undef_locs; auto.
 + (* Lgetstack, outgoing *)
   exploit frame_get_outgoing; eauto. intros (v & A & B).
@@ -2166,6 +2301,7 @@ Proof.
   apply plus_one. apply exec_Mgetstack. exact A.
   econstructor; eauto with coqlib.
   apply agree_regs_set_reg; auto.
+  apply agree_unused_rs_set_reg; eauto.
   apply agree_locs_set_reg; auto.
 
 - (* Lsetstack *)
@@ -2180,8 +2316,8 @@ Proof.
               store_stack m' (Vptr sp' Ptrofs.zero) ty (Ptrofs.repr ofs') (rs0 src) = Some m''
            /\ m'' |= frame_contents f j sp' (Locmap.set (S sl ofs ty) (rs (R src))
                                                (LTL.undef_regs (destroyed_by_setstack ty) rs))
-                                            (parent_locset s) (parent_sp cs') (parent_ra cs')
-                  ** stack_contents j s cs' ** minjection j m ** globalenv_inject se tse j m).
+                                            (parent_locset s)(parent_rs lrs)(parent_sp cs') (parent_ra cs')
+                  ** stack_contents j s cs' lrs ** minjection j m ** globalenv_inject se tse j m).
   { unfold ofs'; destruct sl; try discriminate.
     eapply frame_set_local; eauto.
     eapply frame_set_outgoing; eauto. }
@@ -2210,6 +2346,8 @@ Proof.
     econstructor. eexact STORE. eauto.
   econstructor. eauto. eauto. eauto. eauto.
   apply agree_regs_set_slot. apply agree_regs_undef_regs. auto.
+  eapply agree_unused_rs_undef_regs; eauto.
+  apply destroyed_by_setstack_caller_save.
   apply agree_locs_set_slot. apply agree_locs_undef_locs. auto. apply destroyed_by_setstack_caller_save. auto.
   eauto. eauto with coqlib. eapply is_tail_cons_left. eauto.
   eauto.
@@ -2228,6 +2366,8 @@ Proof.
   econstructor; eauto with coqlib.
   apply agree_regs_set_reg; auto.
   rewrite transl_destroyed_by_op.  apply agree_regs_undef_regs; auto.
+  apply agree_unused_rs_set_reg; eauto.
+  apply agree_unused_rs_undef_regs; auto. apply destroyed_by_op_caller_save.
   apply agree_locs_set_reg; auto. apply agree_locs_undef_locs. auto. apply destroyed_by_op_caller_save.
   apply frame_set_reg. apply frame_undef_regs. exact SEP.
 
@@ -2247,6 +2387,7 @@ Proof.
   apply plus_one. econstructor; eauto.
   econstructor; eauto with coqlib.
   apply agree_regs_set_reg. rewrite transl_destroyed_by_load. apply agree_regs_undef_regs; auto. auto.
+  apply agree_unused_rs_set_reg; auto.
   apply agree_locs_set_reg. apply agree_locs_undef_locs. auto. apply destroyed_by_load_caller_save. auto.
 
 - (* Lstore *)
@@ -2272,16 +2413,17 @@ Proof.
   destruct a; cbn in H0; try congruence.
   rewrite (Mem.support_store _ _ _ _ _ _ H0). eauto.
   rewrite transl_destroyed_by_store. apply agree_regs_undef_regs; auto.
+  apply agree_unused_rs_undef_regs; auto. apply destroyed_by_store_caller_save.
   apply agree_locs_undef_locs. auto. apply destroyed_by_store_caller_save.
   auto. eauto with coqlib.
   rewrite globalenv_support in SEP.
   eapply frame_undef_regs; eauto.
   destruct a; try discriminate. apply Mem.support_store in H0. rewrite H0. eauto.
   etransitivity. eauto. eauto.
-  
+
 - (* Lcall *)
   exploit find_function_translated; eauto.
-    eapply sep_proj2. eapply sep_proj2. eapply sep_proj2. eexact SEP.
+  eapply sep_proj2. eapply sep_proj2. eapply sep_proj2. eexact SEP.
   intros [tf' [A B]].
   exploit is_tail_transf_function; eauto. intros IST.
   rewrite transl_code_eq in IST. simpl in IST.
@@ -2291,16 +2433,18 @@ Proof.
   econstructor; eauto.
   econstructor; eauto with coqlib.
   unfold Val.offset_ptr. destruct fb; constructor; eauto.
+  destruct fb; try inv FIND. simpl. congruence.
   intros; red.
     apply Z.le_trans with (size_arguments (Linear.funsig f')); auto.
     apply loc_arguments_bounded; auto.
-  destruct ros; simpl in *; eauto. eapply symbol_address_inject; eauto. apply SEP.
+    destruct ros; simpl in *; eauto. eapply symbol_address_inject; eauto. apply SEP.
+  reflexivity.
   simpl. rewrite sep_assoc. exact SEP.
-
+  
 - (* Ltailcall *)
-  rewrite (sep_swap (stack_contents j s cs')) in SEP.
+  rewrite (sep_swap (stack_contents j s cs' lrs)) in SEP.
   exploit function_epilogue_correct; eauto. inversion Hm. auto. inv AGLOCS.
-  clear SEP. intros (rs1 & m1' & P & Q & R & S & T & U & SEP).
+  clear SEP. intros (rs1 & m1' & P & Q & R & S & T & U & V & SEP).
   rewrite sep_swap in SEP.
   exploit find_function_translated; eauto.
     eapply sep_proj2. eapply sep_proj2. eexact SEP.
@@ -2335,13 +2479,13 @@ Proof.
   apply zero_size_arguments_tailcall_possible. eapply wt_state_tailcall; eauto.
   eauto.
   destruct ros; simpl in *; eauto. eapply symbol_address_inject; eauto. apply SEP.
-  eauto. 
+  eauto. intros. rewrite <- V; eauto.
   rewrite globalenv_support in SEP. eauto. 
   apply Mem.support_free in H2. rewrite H2. eauto.
   eapply injp_acc_small_implies; eauto.
 
 - (* Lbuiltin *)
-destruct BOUND as [BND1 BND2].
+  destruct BOUND as [BND1 BND2].
   exploit transl_builtin_args_correct.
     eauto. eauto. rewrite sep_swap in SEP; apply sep_proj2 in SEP; eexact SEP. inversion Hm. eauto.
     eauto. rewrite <- forallb_forall. eapply wt_state_builtin; eauto.
@@ -2358,11 +2502,11 @@ destruct BOUND as [BND1 BND2].
   red. intro. eauto using external_call_readonly; eauto.
   red. intro. eauto using external_call_readonly; eauto.
   red. intros. eapply external_call_max_perm; eauto.
-  red. intros. eapply external_call_max_perm; eauto.  
+  red. intros. eapply external_call_max_perm; eauto.
   econstructor; split.
-  apply plus_one. econstructor; eauto.  
+  apply plus_one. econstructor; eauto.
   eapply match_states_intro with (j := j').
-  apply Mem.unchanged_on_support in UNCH1. eauto.  
+  apply Mem.unchanged_on_support in UNCH1. eauto.
   eapply match_stacks_change_meminj. eauto. eauto.
   apply Mem.unchanged_on_support in UNCH1. eauto.
   unfold init_m2.
@@ -2373,14 +2517,14 @@ destruct BOUND as [BND1 BND2].
   (* inv ACCE. destruct H9 as [[_ X] _].  congruence. *)
   (* eapply stack_contents_support; eauto. apply SEP'. *)
   apply agree_regs_set_res; auto. apply agree_regs_undef_regs; auto. eapply agree_regs_inject_incr; eauto.
-  (* apply agree_unused_rs_set_res; auto. apply agree_unused_rs_undef_regs_1; auto. *)
+  apply agree_unused_rs_set_res; auto. apply agree_unused_rs_undef_regs_1; auto.
   apply agree_locs_set_res; auto. apply agree_locs_undef_regs; auto.
   eauto. eauto. eauto with coqlib.
   apply frame_set_res. apply frame_undef_regs. apply frame_contents_incr with j; auto.
   rewrite sep_swap2. apply stack_contents_change_meminj with j; auto. rewrite sep_swap2.
   exact SEP.
   etransitivity. eauto. eauto.
-  
+
 - (* Llabel *)
   econstructor; split.
   apply plus_one; apply exec_Mlabel.
@@ -2400,6 +2544,7 @@ destruct BOUND as [BND1 BND2].
   eapply transl_find_label; eauto.
   econstructor. eauto. eauto. eauto. eauto.
   apply agree_regs_undef_regs; auto.
+  apply agree_unused_rs_undef_regs. auto. apply destroyed_by_cond_caller_save.
   apply agree_locs_undef_locs. auto. apply destroyed_by_cond_caller_save.
   auto. eauto.
   eapply find_label_tail; eauto.
@@ -2411,6 +2556,7 @@ destruct BOUND as [BND1 BND2].
   eapply eval_condition_inject with (m1 := m). eapply agree_reglist; eauto. apply sep_pick3 in SEP; exact SEP. auto.
   econstructor. eauto. eauto. eauto. eauto.
   apply agree_regs_undef_regs; auto.
+  apply agree_unused_rs_undef_regs. auto. apply destroyed_by_cond_caller_save.
   apply agree_locs_undef_locs. auto. apply destroyed_by_cond_caller_save.
   auto. eauto. eauto with coqlib.
   apply frame_undef_regs; auto. eauto.
@@ -2423,14 +2569,15 @@ destruct BOUND as [BND1 BND2].
   apply transl_find_label; eauto.
   econstructor. eauto. eauto. eauto. eauto.
   apply agree_regs_undef_regs; auto.
+  apply agree_unused_rs_undef_regs. auto. apply destroyed_by_jumptable_caller_save.
   apply agree_locs_undef_locs. auto. apply destroyed_by_jumptable_caller_save.
   auto. eauto. eapply find_label_tail; eauto.
   apply frame_undef_regs; auto. eauto.
 
 - (* Lreturn *)
-  rewrite (sep_swap (stack_contents j s cs')) in SEP.
+  rewrite (sep_swap (stack_contents j s cs' lrs)) in SEP.
   exploit function_epilogue_correct; eauto.
-  intros (rs' & m1' & A & B & C & D & E & F & G).
+  intros (rs' & m1' & A & B & C & D & E & F & SAVE & G).
   assert (Hm': Mem.inject j m' m1').
   apply G.
   assert (ACC1: injp_acc_small init_wj (injpw j m m'0 Hm) (injpw j m' m1' Hm')).
@@ -2457,11 +2604,12 @@ destruct BOUND as [BND1 BND2].
   eapply plus_right. eexact D. econstructor; eauto. traceEq.
   econstructor; eauto.
   rewrite (Mem.support_free _ _ _ _ _ H); eauto.
+  intros. rewrite <- SAVE; eauto.
   rewrite globalenv_support in G.
   rewrite sep_swap; exact G.
   apply Mem.support_free in H. rewrite H. eauto.
   eapply injp_acc_small_implies. eauto. eauto.
-  
+
 - (* internal function *)
   rewrite FIND in FIND0. inv FIND0.
   edestruct functions_translated as (tf & TFIND & TRANSL); eauto. apply SEP.
@@ -2476,7 +2624,7 @@ destruct BOUND as [BND1 BND2].
   eapply match_stacks_type_sp; eauto.
   eapply match_stacks_type_retaddr; eauto.
   clear SEP;
-  intros (j' & rs' & m2' & sp' & m3' & m4' & m5' & Hm' & A & B & C & D & E & E2 & SEP & J & K & L & M).
+  intros (j' & rs' & m2' & sp' & m3' & m4' & m5' & Hm' & A & B & C & D & E & E' & F & SEP & J & K & L & M).
   rewrite (sep_comm (globalenv_inject se tse j' m')) in SEP.
   rewrite (sep_swap (minjection j' m')) in SEP.
   econstructor; split.
@@ -2487,15 +2635,18 @@ destruct BOUND as [BND1 BND2].
   rewrite (Mem.support_alloc _ _ _ _ _ H); eauto.
   eapply match_stacks_change_meminj; eauto.
   eapply stack_contents_support; eauto. apply SEP'.
+  red. intros. rewrite F; eauto. apply TRS.
+  eapply reg_within_bounds_caller_save; eauto.
   unfold init_m1, init_m2. inv ACC. 
   split. intro. eapply Mem.fresh_block_alloc. apply H.
-  eapply Mem.valid_block_unchanged_on; eauto. 
+  eapply Mem.valid_block_unchanged_on; eauto.
   intro. eapply Mem.fresh_block_alloc; eauto.
   eapply Mem.valid_block_unchanged_on; eauto.
   rewrite sep_swap in SEP.
+  eapply frame_callee_save_eq; eauto.
   rewrite sep_swap. eapply stack_contents_change_meminj; eauto.
   etransitivity. eauto. eauto.    
-
+  
 - (* external function *)
   rewrite FIND in FIND0. inv FIND0.
   edestruct functions_translated as (tf & TFIND & TRANSL); eauto. apply SEP.
@@ -2509,9 +2660,9 @@ destruct BOUND as [BND1 BND2].
   assert (Hm': Mem.inject j' m' m1'). apply E.
   assert (ACC1: injp_acc (injpw j m m'0 Hm) (injpw j' m' m1' Hm')).
   { econstructor; eauto.
-    red. intro. eauto using external_call_readonly; eauto.
-    red. intro. eauto using external_call_readonly; eauto.
-    red. intros. eapply external_call_max_perm; eauto.
+  red. intro. eauto using external_call_readonly; eauto.
+  red. intro. eauto using external_call_readonly; eauto.
+  red. intros. eapply external_call_max_perm; eauto.
     red. intros. eapply external_call_max_perm; eauto.  }
   econstructor; split.
   apply plus_one. eapply exec_function_external; eauto.
@@ -2523,21 +2674,29 @@ destruct BOUND as [BND1 BND2].
   apply agree_regs_set_pair. apply agree_regs_undef_caller_save_regs.
   apply agree_regs_inject_incr with j; auto.
   auto.
+  intros. 
+  transitivity ((undef_caller_save_regs rs) r).
+  generalize (CallConv.loc_result_always_one (ef_sig ef)).
+  intros [r0 Hr]. rewrite Hr. simpl. rewrite Regmap.gso. reflexivity.
+  generalize (loc_result_caller_save (ef_sig ef)).
+  intro Hcs. rewrite Hr in Hcs. simpl in Hcs. congruence.
+  unfold undef_caller_save_regs. rewrite H. eauto.
+  
   apply stack_contents_change_meminj with j; auto.
   rewrite sep_comm, sep_assoc; auto.
   etransitivity. eauto. eauto.
-  
+
 - (* return *)
   inv STACKS. exploit wt_returnstate_agree; eauto. intros [AGCS OUTU].
   simpl in AGCS. simpl in SEP. rewrite sep_assoc in SEP.
   econstructor; split.
   apply plus_one. apply exec_return.
   econstructor; eauto.
-  (* red. intros. red in AGRS. simpl in CALLEESAVE. rewrite CALLEESAVE. *)
-  (* eauto. destruct (is_callee_save r) eqn:Hcs. reflexivity. *)
-  (* elim H. red. intros. congruence. *)
-  apply agree_locs_return with rs0; auto. 
-  eapply frame_contents_exten with rs0 (parent_locset s); auto.
+  red. intros. red in AGRS. simpl in CALLEESAVE. rewrite CALLEESAVE.
+  eauto. destruct (is_callee_save r) eqn:Hcs. reflexivity.
+  elim H. red. intros. congruence.
+  apply agree_locs_return with rs0; auto.
+  eapply frame_contents_exten with rs0 (parent_locset s) (parent_rs lrs'); auto.
   intros; apply Val.lessdef_same; apply AGCS; red; congruence.
   intros; rewrite (OUTU ty ofs); auto.
 Qed.
@@ -2573,6 +2732,7 @@ Proof.
   symmetry. apply loc_external_is. constructor; auto.
 Qed.
 
+
 Lemma transf_initial_states:
   forall w q1 q2, match_senv ccB w se tse -> match_query ccB w q1 q2 ->
   forall st1, Linear.initial_state ge q1 st1 -> (* wt_locset (lq_rs q1) -> *)
@@ -2586,17 +2746,14 @@ Proof.
   - (* rename f0 into j. rename m into m1. *)
     eapply match_states_call; eauto.
     + constructor; auto. cbn. congruence.
-    (* + reflexivity. *)
+    + reflexivity.
     + cbn [stack_contents stk_sg stk_sp2 stk_m2].
       subst rs0. rewrite <- init_args_initial_regs.
       rewrite <- sep_assoc. repeat (apply conj; auto).
-      (* * tinv. *)
       * intros b ofs Hofs (b0 & delta & Hb & Hp). eapply H11; eauto.
       * intros ? ?. cbn. auto.
     + simpl. reflexivity.
-    (* + simpl. reflexivity. *)
 Qed.
-
 
 Lemma transf_final_states:
   forall w st1 st2 r1, wt_state prog se st1 -> match_states w st1 st2 -> Linear.final_state st1 r1 ->
@@ -2609,7 +2766,7 @@ Proof.
     cbn [stack_contents] in SEP. rewrite ! and_assoc in SEP.
     destruct SEP as (UNC1 & ARGS & VINJ & MINJ & GINJ & SUP1 & SUP2 & DISJ & DIS2).
     eapply cc_stacking_mr_intro; cbn; eauto.
-    + intros r Hr. simpl in *. setoid_rewrite <- (AGCS (R r) Hr); eauto.
+    + intros r Hr. simpl in *. erewrite <- CALLEESAVE; eauto.
     + intros sb2 sofs2 H sb1 delta Hsb Hp. eapply DIS2; cbn; eauto.
 Qed.
 
@@ -2629,13 +2786,12 @@ Lemma transf_external_states:
   forall r1 r2 st1', match_reply ccA wx r1 r2 -> Linear.after_external ge st1 r1 st1' ->
   exists st2', Mach.after_external st2 r2 st2' /\ match_states w st1' st2'.
 Proof.
-  
   intros w st1 st2 q1 WTS Hst Hq1. destruct Hst; inv Hq1.
   inv WTS. rewrite FIND in H4; inv H4. fold ge in FIND0. rewrite FIND in FIND0; inv FIND0.
   edestruct functions_translated as (tf & TFIND & TRANSL); eauto. apply SEP.
   simpl in TRANSL. inv TRANSL.
   assert (MINJ: Mem.inject j m m') by apply SEP.
-  eexists (stkw injp (injpw _ _ _ MINJ) _ ls (parent_sp cs') m'), _. repeat apply conj.
+  eexists (stkw injp (injpw _ _ _ MINJ) _ ls rs (parent_sp cs') m'), _. repeat apply conj.
   - econstructor; eauto.
   - eapply match_stacks_init_args in SEP; eauto.
     econstructor; eauto.
@@ -2647,17 +2803,19 @@ Proof.
     + eapply match_stacks_type_sp; eauto.
     + eapply match_stacks_type_retaddr; eauto.
   - constructor; apply SEP.
-  - intros r1 r2 st1' Hr Hst1'. inv Hr. inv H4. inv Hst1'. inv H9.
+  - intros r1 r2 st1' Hr Hst1'. inv Hr. inv H5. inv Hst1'. inv H10.
     rewrite H19 in FIND. inv FIND.
     eexists. split.
     + econstructor; eauto.
-    + eapply match_states_return with (j := f'); eauto.
-      * eauto.
-        apply Mem.unchanged_on_support in H12; eauto.
+    + eapply match_states_return with (j := f').
+      * apply Mem.unchanged_on_support in H7.
+        eapply Mem.sup_include_trans. eauto. auto.
       * eapply match_stacks_change_meminj; eauto.
         eapply stack_contents_support; eauto. apply SEP.
       * intros r. cbn. destruct in_dec; eauto.
         destruct is_callee_save eqn:Hr; eauto.
+        rewrite <- H9. eauto. eauto.
+      * intros. rewrite <- H9; eauto.
       * eapply stack_contents_change_meminj; eauto.
         rewrite sep_comm, sep_assoc in SEP |- *.
         eapply minjection_incr; eauto.
